examples/src/exponential.ml
@@ -4,3 +4,8 @@ let rec f n =
     f (n-1);
     f (n-1)
   end
+
+let loop n =
+  for i = 0 to n-1 do
+    f i
+  done
