examples/proofs/Dichotomy_proof.v
@@ -18,6 +18,8 @@ Require Import elia.
 (* Load the CF definitions. *)
 Require Import Dichotomy_ml.
 
+Require Import Sorted.
+
 Ltac auto_tilde ::= try solve [ auto with maths | false; math ].
 
 Lemma middle_inbound : forall i j m,
@@ -40,14 +42,98 @@ Qed.
 
 Hint Resolve half_pos.
 
+Definition bsearch_correct (xs: list int) v i j k :=
+     (k = -1 /\ forall p, i <= p < j -> xs[p] <> v)
+  \/ (i <= k < j /\ xs[k] = v).
+
+Lemma bsearch_correct_oob xs v i j :
+  j <= i ->
+  bsearch_correct xs v i j (-1).
+Proof. intros. left~. Qed.
+
+Hint Resolve bsearch_correct_oob.
+
+Lemma bsearch_correct_found xs v i j k :
+  i <= k < j ->
+  v = xs[k] ->
+  bsearch_correct xs v i j k.
+Proof. intros. right~. Qed.
+
+Hint Resolve bsearch_correct_found.
+
+Lemma sort_read : forall l,
+  LocallySorted Z.le l ->
+  forall i j,
+  0 <= i ->
+  i <= j ->
+  j < length l ->
+  l[i] <= l[j].
+Proof.
+  induction 1.
+  { intros. false. rew_list in *. math. }
+  { intros. rew_list in *. rew_array. repeat case_if~. }
+  { intros. rew_list in *. rew_array.
+    case_if.
+    { case_if~. case_if~.
+      transitivity b. auto.
+      specializes IHLocallySorted 0 (j-1) __ __ __.
+      rew_array in *. case_if~. case_if~. }
+    { case_if~.
+      { case_if~. case_if~.
+        specializes IHLocallySorted 0 (j-1) __ __ __.
+        rew_array in *. repeat case_if~. }
+      { case_if~. case_if~.
+        specializes IHLocallySorted (i-1) (j-1) __ __ __.
+        rew_array in *. repeat case_if~. } } }
+Qed.
+
+Lemma bsearch_correct_recurse_l xs v i j j' k :
+  LocallySorted Z.le xs ->
+  0 <= i -> j <= length xs ->
+  i <= j' < j ->
+  v < xs[j'] ->
+  bsearch_correct xs v i j' k ->
+  bsearch_correct xs v i j k.
+Proof.
+  intros S Hi Hj Hij Hv C.
+  assert (Hsort: forall p, j' <= p < j -> v < xs[p]).
+  { intros. forwards~: sort_read xs j' p. }
+  destruct C as [(-> & C)|(Hk & C)].
+  { left~. split~. intros.
+    specializes C p. specializes Hsort p.
+    tests: (p < j'). specializes~ C __. specializes~ Hsort __; autos~. }
+  { right~. }
+Qed.
+
+Lemma bsearch_correct_recurse_r xs v i i' j k :
+  LocallySorted Z.le xs ->
+  0 <= i -> j <= length xs ->
+  i <= i' < j ->
+  xs[i'] < v ->
+  bsearch_correct xs v (i'+1) j k ->
+  bsearch_correct xs v i j k.
+Proof.
+  intros S Hi Hj Hij Hv C.
+  assert (Hsort: forall p, i <= p <= i' -> xs[p] < v).
+  { intros. forwards~: sort_read xs p i'. }
+  destruct C as [(-> & C)|(Hk & C)].
+  { left~. split~. intros.
+    tests: (p <= i'). { specializes Hsort p __. }
+    specializes C p __. }
+  { right~.  }
+Qed.
+
 Lemma bsearch_spec :
   specZ [cost \in_O Z.log2]
     (forall t (xs : list int) (v : int) (i j : int),
+        LocallySorted Z.le xs ->
         0 <= i <= length xs ->
         0 <= j <= length xs ->
         app bsearch [t v i j]
         PRE (\$ (cost (j - i)) \* t ~> Array xs)
-        POST (fun (k:int) => t ~> Array xs)).
+        POST (fun (k:int) =>
+                t ~> Array xs \*
+                \[ bsearch_correct xs v i j k ])).
 Proof.
   begin defer assuming a b.
   defer Ha: (0 <= a).
@@ -70,23 +156,28 @@ Proof.
 
   { xspecO cost.
     introv. gen_eq n: (j-i). gen i j. induction_wf IH: (downto 0) n.
-    intros i j Hn Hi Hj.
+    intros i j Hn Hxs Hi Hj.
 
     weaken. xcf. xpay.
     (* xif_ifcost / xif_maxcost / xif = celui qui sert le plus souvent *)
     xif_guard as C. { xret~. }
+
     (* rewrite nle_as_gt in C. *) asserts~ C' : (i < j). clear C.
     xret ;=> Hm. forwards~ Hmbound: middle_inbound Hm.
     xapps. { apply~ int_index_prove. }
     xrets. xif. { xret~. }
     xapps. { apply~ int_index_prove. }
     xif.
-    { weaken. xapp~ (m - i). subst m.
+    { weaken. xapp~ (m - i).
+      hsimpl. applys~ bsearch_correct_recurse_l m.
+      subst m.
       (* tactique xcost? *)
       match goal with |- cost ?x <= _ => ring_simplify x end.
       reflexivity. }
     { (* forwards: IH __ (m+1) j. Focus 2. reflexivity. *)
-      weaken. xapp~ (j - (m+1)). subst m. reflexivity. }
+      weaken. xapp~ (j - (m+1)).
+      hsimpl. applys~ bsearch_correct_recurse_r m.
+      subst m. reflexivity. }
 
     cases_if; ring_simplify.
     { rewrite~ costPneg. }
@@ -106,7 +197,6 @@ Proof.
         rewrite ZP. exists 1. intros. cases_if~.
       - dominated. }
   }
-
   end defer. elia.
 Qed.
 
@@ -144,31 +234,70 @@ Proof.
       rewrite (Z.max_r 0); [| auto with zarith].
       rewrite Z.max_l; swap 1 2.
       { apply M. forwards~: Zquot_mul_2 (j-i). }
-      tests Hn1: (j-i = 1).
-      + rewrite Hn1. cbn. asserts_rewrite~ (n = 1). defer.
-      + assert (HH: 2 <= n) by math. rewrite <-Hn.
-        generalize n HH. defer. }
-  }
+      assert (HH: 1 <= n) by math. rewrite <-Hn.
+      generalize n HH. defer. } }
 
   close_cost.
 
-  begin defer assuming a b.
-  defer Ha: (0 <= a).
-  exists (fun (n:Z_filterType) => If 0 < n then a * Z.log2 n + b else 1).
+  begin defer assuming a b c.
+  exists (fun (n:Z_filterType) => If 0 < n then a * Z.log2 n + b else c).
   repeat split.
-  { intros. cases_if~. }
-  { intros. cases_if~. rewrite <-Z.log2_nonneg. pols. defer. }
-  { cases_if~. cases_if~. simpl. pols. defer. }
-  { intros n N. cases_if~; [| now false~]. cases_if~.
-    rewrite~ <-(@Zlog2_step n). pols. defer. }
+  { intros. cases_if~. defer. }
+  { intros. deferred;=>. cases_if~. rewrite <-Z.log2_nonneg. pols. all: defer. }
+  { intros n N. tests: (n = 1).
+    { repeat cases_if~. cbn. pols. defer. }
+    { cases_if~; [| now false~]. cases_if~. rewrite~ <-(@Zlog2_step n). pols.
+      defer. } }
 
   cleanup_cost.
   { intros x y H. cases_if; case_if~.
-    { monotonic. }
-    { rewrite <-Z.log2_nonneg. pols. deferred; math. } }
+    { deferred. monotonic. }
+    { rewrite <-Z.log2_nonneg. 2: now deferred. pols. deferred; math. } }
   { transitivity (fun x => a * Z.log2 x + b).
     - apply dominated_ultimately_eq.
       rewrite ZP. exists 1. intros. cases_if~.
     - dominated. }
-  end defer. elia.
+  end defer. elia. (* a = 3, b = 4, c = 1 *)
+Qed.
+
+Ltac r2l := credr2l; apply pred_incl_refl.
+
+Require Import ssreflect.
+
+Lemma bsearch_spec_explicit :
+  forall t (xs : list int) (v : int) (i j : int),
+    0 <= i <= length xs ->
+    0 <= j <= length xs ->
+    app bsearch [t v i j]
+    PRE (\$ (If j <= i then 1 else 3 * Z.log2 (j - i) + 4) \* t ~> Array xs)
+    POST (fun (k:int) => t ~> Array xs).
+Proof.
+    introv. gen_eq n: (j-i). gen i j. induction_wf IH: (downto 0) n.
+    intros i j Hn Hi Hj.
+    xcf. xpay. r2l.
+    xif as C.
+    { xret~. case_if~. rewrite credits_join_eq. hsimpl. rewrite le_zarith. pols. math. }
+    asserts~ C': (i < j). clear C. case_if~.
+    xret;=> Hm. forwards~: middle_inbound Hm.
+    xapps. { apply~ int_index_prove. } r2l.
+    xrets. xif.
+    { xret~. rewrite !credits_join_eq. hsimpl. rewrite le_zarith. pols.
+      rewrite -Z.log2_nonneg //. }
+    xapps. { apply~ int_index_prove. } r2l.
+    rewrite !credits_join_eq. match goal with |- context [ \$ ?x ] => ring_simplify x end.
+    xif.
+    { xapp~ (m - i). hsimpl_credits. rewrite le_zarith.
+      apply Zle_minus_le_0. rewrite Hm. rewrite Z.add_simpl_l.
+      tests Hn1: (j-i=1).
+      + rewrite Hn1. cbn. rewrite Z.add_0_r. case_if~. rewrite -Z.log2_nonneg //.
+      + assert (HH: 2 <= n) by math. case_if~. { exfalso. forwards~: half_pos (j-i). }
+        rewrite -Hn. rewrite -(@Zlog2_step n) //. math. }
+    { xapp~ (j - (m+1)). hsimpl_credits. rewrite le_zarith.
+      apply Zle_minus_le_0. rewrite Hm.
+      tests Hn1: (j-i=1).
+      + rewrite Hn1. cbn. case_if~. rewrite -Z.log2_nonneg //.
+      + assert (HH: 2 <= n) by math. rewrite -Hm. case_if. now rewrite -Z.log2_nonneg //.
+        pols. rewrite Hm. forwards~: Zquot_mul_2 (j-i).
+        rewrite -(@Zlog2_step n) //. rewrite Hn. pols.
+        apply~ Z.mul_le_mono_nonneg_l. apply Z.log2_le_mono. math. }
 Qed.
