examples/proofs/Bellman_ford_proof.v
@@ -28,7 +28,7 @@ Definition ZZle (p1 p2 : Z * Z) :=
   let (x2, y2) := p2 in
   1 <= x1 <= x2 /\ 0 <= y1 <= y2.
 
-Lemma bellman_ford2_spec :
+Lemma bellman_ford_spec :
   specO
     (product_filterType Z_filterType Z_filterType)
     ZZle
@@ -36,7 +36,7 @@ Lemma bellman_ford2_spec :
       forall (inf source : int) t (edges : list (int * int * int)%type) (nb_nodes : int),
         0 <= source < nb_nodes ->
         1 <= nb_nodes ->
-        app bellman_ford2 [inf source t nb_nodes]
+        app bellman_ford [inf source t nb_nodes]
         PRE (\$ (cost (nb_nodes, LibListZ.length edges)) \* t ~> Array edges)
         POST (fun (_: array int) => t ~> Array edges))
     (fun '(n,m) => n * m).
@@ -47,31 +47,33 @@ Proof.
   xapp~. apply index_make. apply~ int_index_prove.
   xseq.
 
-  { xfor_inv (fun (_:int) => Hexists (ds: list int), t ~> Array edges \* d ~> Array ds). math.
+  { xfor_inv (fun (_:int) =>
+      Hexists (ds: list int), t ~> Array edges \* d ~> Array ds). math.
     { intros i Hi. xpay.
       xpull. intros ds.
-
       xapp as edges_nb. intro Hedges_nb.
-      weaken. xfor_inv (fun (_:int) => Hexists (ds: list int), t ~> Array edges \* d ~> Array ds). math.
+      weaken. xfor_inv (fun (_:int) =>
+        Hexists (ds: list int), t ~> Array edges \* d ~> Array ds). math.
       { intros j Hj. xpull. intros ds'.
         xpay. xapps. apply~ int_index_prove.
         xmatch.
         xapp as d1. admit. (* TODO *) intro Hd1.
         xapp as d2. admit. (* TODO *) intro Hd2.
         xapp. admit. (* TODO *) }
-      { hsimpl. } { hsimpl. }
-
+      1,2: now hsimpl.
       { subst edges_nb.
         match goal with |- cumul _ _ (fun _ => ?x) <= _ => ring_simplify x end.
-        sets edges_nb: (LibListZ.length edges). (* workaround *)
-        reflexivity. }
+        sets edges_nb: (LibListZ.length edges). reflexivity. }
     }
     { hsimpl. }
   }
   { xpull. intros ds. xret. hsimpl. }
   cleanup_cost.
 
-  admit. (* TODO monotonic *)
+  { equates 1; swap 1 2.
+    { instantiate (1 := (fun '(x, y) => _)). apply fun_ext_1. intros [x y].
+      rewrite !cumul_const'. rew_cost. reflexivity. }
+    intros [x1 y1] [x2 y2] [H1 H2]. math_nia. }
 
   apply_nary dominated_sum_distr_nary; swap 1 2.
   dominated.
@@ -84,30 +86,18 @@ Proof.
   { eapply dominated_transitive.
     apply dominated_product_swap.
     apply Product.dominated_big_sum_bound_with.
-    { (* ultimately_greater. *) (* FIXME *) admit. }
+    { apply filter_universe_alt. intros. rewrite~ <-cumul_nonneg. math_lia. }
     { monotonic. }
     { limit. (* FIXME *) apply limit_sum_cst_r. limit. }
-
     simpl. dominated.
 
-    apply_nary dominated_sum_distr_nary.
-    { apply_nary dominated_sum_distr_nary.
-      { reflexivity. }
-      { dominated. } }
-    { dominated. }
-
-    apply_nary dominated_sum_distr_nary.
-    { dominated. }
-    { apply_nary dominated_sum_distr_nary.
-      { dominated. }
-      { dominated.
-        eapply dominated_transitive.
-        apply Product.dominated_big_sum_bound.
-        { ultimately_greater. } { monotonic. }
-        simpl. dominated. } } }
+    now repeat apply_nary dominated_sum_distr_nary; dominated.
+    repeat apply_nary dominated_sum_distr_nary; dominated.
+    etransitivity. apply Product.dominated_big_sum_bound.
+    ultimately_greater. monotonic. dominated.
 Admitted.
 
-Lemma bellman_ford2_spec_within :
+Lemma bellman_ford_spec_within :
   specO
     (within_filterType (product_filterType Z_filterType Z_filterType)
       (fun '(n,m) => m <= n^2))
@@ -116,14 +106,14 @@ Lemma bellman_ford2_spec_within :
       forall (inf source : int) t (edges : list (int * int * int)%type) (nb_nodes : int),
         0 <= source < nb_nodes ->
         1 <= nb_nodes ->
-        app bellman_ford2 [inf source t nb_nodes]
+        app bellman_ford [inf source t nb_nodes]
         PRE (\$ (cost (nb_nodes, LibListZ.length edges)) \* t ~> Array edges)
         POST (fun (_: array int) => t ~> Array edges))
     (fun '(n,m) => n ^ 3).
 Proof.
-  econstructor; try (intros; apply~ bellman_ford2_spec).
+  econstructor; try (intros; apply~ bellman_ford_spec).
   eapply dominated_transitive.
-  { destruct (cost_dominated bellman_ford2_spec) as [c U].
+  { destruct (cost_dominated bellman_ford_spec) as [c U].
     exists c. applys within_finer U. }
   { exists 1. rewrite withinP.
     rewrite productP. do 2 exists (fun x => 0 <= x).
@@ -134,24 +124,24 @@ Proof.
     rewrite D. math_nia. }
 Qed.
 
-Lemma bellman_ford2_spec_derived :
+Lemma bellman_ford_spec_derived :
   specZ [cost \in_O (fun n => n^3)] (
     forall (inf source : int) t (edges : list (int * int * int)%type) (nb_nodes : int),
       0 <= source < nb_nodes ->
       1 <= nb_nodes ->
       LibListZ.length edges <= nb_nodes ^ 2 ->
-      app bellman_ford2 [inf source t nb_nodes]
+      app bellman_ford [inf source t nb_nodes]
       PRE (\$ (cost nb_nodes) \* t ~> Array edges)
       POST (fun (_: array int) => t ~> Array edges)).
 Proof.
   xspecO (fun n =>
     let m := If 0 < n then n^2 else 0 in
     let n' := If 0 < n then n else 1 in
-    cost bellman_ford2_spec (n', m)).
-  { introv Hnodes Hedges. intros; xapply~ (spec bellman_ford2_spec).
+    cost bellman_ford_spec (n', m)).
+  { introv Hnodes Hedges. intros; xapply~ (spec bellman_ford_spec).
     hsimpl_credits. (* FIXME *)
     match goal with |- le 0 (?x - ?y) => enough (y <= x) by math end.
-    apply (cost_monotonic bellman_ford2_spec).
+    apply (cost_monotonic bellman_ford_spec).
     unfolds ZZle. splits~. cases_if~. cases_if~.
   }
   { eapply monotonic_comp. monotonic.
@@ -163,7 +153,7 @@ Proof.
     eapply dominated_ultimately_eq.
     { exists 1. intros. cases_if~. reflexivity. }
     eapply dominated_comp_eq.
-    apply (cost_dominated bellman_ford2_spec).
+    apply (cost_dominated bellman_ford_spec).
     2: intro; reflexivity.
     2: intro; reflexivity.
     limit. }
